rupicola/refinements2/OldCompilableWP.fst
@@ -1,0 +1,367 @@
+module OldCompilableWP
+
+open FStar.Tactics
+
+(** Helpers to deal with Monotonicity of Pure **)
+module M = FStar.Monotonic.Pure
+
+let intro_pure_wp_monotonicity (#a:Type) (wp:pure_wp' a)
+  : Lemma
+      (requires M.is_monotonic wp)
+      (ensures pure_wp_monotonic a wp)
+    [SMTPat (pure_wp_monotonic a wp)]
+  = M.intro_pure_wp_monotonicity wp
+
+unfold let (<=) #a (wp1 wp2:pure_wp a) = pure_stronger a wp1 wp2
+unfold let ret #a x : pure_wp a = pure_return a x //fun p -> p x
+
+(** Typing environment **)
+type env = var -> option Type0
+let empty : env = fun _ -> None
+
+(* we only need extend at 0 *)
+let extend (t:Type0) (g:env)
+  : env
+  = fun y -> if y = 0 then Some t
+          else g (y-1)
+
+(** F* evaluation environment **)
+assume val fs_env (g:env) : Type u#0
+assume val fs_empty : fs_env empty
+assume val get_v : #g:env -> fs_env g -> x:var{Some? (g x)} -> Some?.v (g x)
+assume val fs_extend : #g:env -> fsG:fs_env g -> #t:Type0 -> t -> fs_env (extend t g)
+assume val fs_shrink : #t:Type0 -> #g:env -> fs_env (extend t g) -> fs_env g
+
+type spec_env (g:env) (a:Type) =
+  fsG:fs_env g -> pure_wp a
+
+(** Definition of open FStar expressions **)
+type fs_oexp (g:env) (a:Type) (wpG:spec_env g a) =
+  fsG:fs_env g -> PURE a (wpG fsG) // <= ret x} (** this works better than using PURE **)
+
+unfold
+val wp_ref :
+  #g:env ->
+  #a:Type ->
+  ref1:(a -> Type0) ->
+  ref2:(a -> Type0) ->
+  wpV:spec_env g (x:a{ref1 x}) ->
+  spec_env g (x:a{ref2 x})
+let wp_ref #g #a ref1 ref2 wpV =
+  FStar.Monotonic.Pure.elim_pure_wp_monotonicity_forall ();
+  fun fsG (p:pure_post (x:a{ref2 x})) ->
+    wpV fsG (fun r -> ref2 r /\ p r)
+
+unfold
+val helper_ref : #g:env ->
+                 #a:Type ->
+                 #ref1:(a -> Type0) ->
+                 #ref2:(a -> Type0) ->
+                 #wpV:spec_env g (x:a{ref1 x}) ->
+                 v:fs_oexp g (x:a{ref1 x}) wpV ->
+                 fs_oexp g (x:a{ref2 x}) (wp_ref ref1 ref2 wpV)
+let helper_ref #g #a #ref1 #ref2 #wpV v =
+  FStar.Monotonic.Pure.elim_pure_wp_monotonicity_forall ();
+  fun fsG -> v fsG
+
+unfold
+val wp_lambda : #g :env ->
+                #a :Type ->
+                #b :Type ->
+                wpBody:spec_env (extend a g) b ->
+                spec_env g (a -> b)
+
+let wp_lambda #g #a #b wpBody fsG : pure_wp (a -> b) =
+  fun (p:pure_post (a -> b)) ->
+    forall (f:a -> b).
+      (forall (p':pure_post b) (fsG':fs_env (extend a g)).
+        fsG == fs_shrink fsG' ==>  wpBody fsG' p' ==>  p' (f (get_v fsG' 0))
+      ) ==>  p f
+(**
+ //  (forall f. p f) ==>
+ //    (forall x. wpBody (fs_extend fsG x) (fun _ -> True)) /\
+ //    (forall f. ret f p)
+
+
+  //  forall (fsG':fs_env (extend a g)). fsG == fs_shrink fsG' ==>
+  //    wpBody fsG' (fun r -> forall f. f fsG' (get_v fsG' 0) == r /\ p (f fsG'))
+**)
+
+unfold
+val helper_lambda : #g :env ->
+                    #a :Type ->
+                    #b :Type ->
+                    wpBody:spec_env (extend a g) b ->
+                    f :fs_oexp g (a -> b) (wp_lambda wpBody) ->
+                    fs_oexp (extend a g) b wpBody
+let helper_lambda #g #a #b wpBody f : fs_oexp (extend a g) b wpBody =
+  fun fsG -> f (fs_shrink #a fsG) (get_v fsG 0)
+
+unfold
+val helper_var : g:env ->
+                 a:Type ->
+                 x:var{Some? (g x) /\ a == Some?.v (g x)} ->
+                 fs_oexp g a (fun fsG p -> p (get_v fsG x))
+let helper_var g a x fsG = get_v fsG x
+
+unfold
+val helper_var1 : g:env ->
+                  a:Type ->
+                  b:Type ->
+                  x:var{Some? (g x) /\ a == Some?.v (g x)} ->
+                  fs_oexp (extend b g) a (fun fsG p -> p (get_v (fs_shrink #b fsG) x))
+let helper_var1 g a b x fsG = get_v (fs_shrink #b fsG) x
+
+unfold
+val helper_var2 : g:env ->
+                  a:Type ->
+                  b:Type ->
+                  c:Type ->
+                  x:var{Some? (g x) /\ a == Some?.v (g x)} ->
+                  fs_oexp (extend c (extend b g)) a (fun fsG p -> p (get_v (fs_shrink #b (fs_shrink #c fsG)) x))
+let helper_var2 g a b c x fsG = get_v (fs_shrink #b (fs_shrink #c fsG)) x
+
+unfold
+val fapp_wp : #g :env ->
+              #a :Type ->
+              #b :Type ->
+              wpF : spec_env g (a -> b) ->
+              wpX : spec_env g a ->
+              spec_env g b
+let fapp_wp #g #a #b wpF wpX fsG : pure_wp b =
+  FStar.Monotonic.Pure.elim_pure_wp_monotonicity_forall ();
+  fun (p:pure_post b) -> wpF fsG (fun f' -> wpX fsG (fun x' -> p (f' x')))
+
+unfold
+val helper_fapp : g :env ->
+                  a :Type ->
+                  b :Type ->
+                  wpF : spec_env g (a -> b) ->
+                  f :fs_oexp g (a -> b) wpF ->
+                  wpX : spec_env g a ->
+                  x :fs_oexp g a wpX ->
+                  fs_oexp g b (fapp_wp wpF wpX)
+
+let helper_fapp g a b wpF f wpX x : fs_oexp g b (fapp_wp wpF wpX) =
+  FStar.Monotonic.Pure.elim_pure_wp_monotonicity_forall ();
+  fun fsG -> (f fsG) (x fsG)
+
+unfold
+val if_wp : #g :env ->
+            #a :Type ->
+            wpC : spec_env g bool ->
+            wpT : spec_env g a ->
+            wpE : spec_env g a ->
+            spec_env g a
+let if_wp #g #a wpC wpT wpE fsG : pure_wp a =
+  FStar.Monotonic.Pure.elim_pure_wp_monotonicity_forall ();
+  fun (p:pure_post a) ->
+    wpC fsG (fun r -> (r == true ==> wpT fsG p) /\ (r == false ==> wpE fsG p))
+
+unfold
+val helper_if : #g :env ->
+                #a :Type ->
+                #wpC : spec_env g bool ->
+                c   : fs_oexp g bool wpC ->
+                #wpT : spec_env g a ->
+                t   : fs_oexp g a wpT ->
+                #wpE : spec_env g a ->
+                e   : fs_oexp g a wpE ->
+                fs_oexp g a (if_wp wpC wpT wpE)
+let helper_if c t e fsG =
+  FStar.Monotonic.Pure.elim_pure_wp_monotonicity_forall ();
+  if c fsG then t fsG else e fsG
+
+unfold
+val wp_seq :     #g:env ->
+                 ref1:Type0 ->
+                 wpV:spec_env g (x:unit{ref1}) ->
+                 #a:Type ->
+                 wpK:spec_env g a ->
+                 spec_env g a
+let wp_seq ref1 wpV wpK fsG =
+  FStar.Monotonic.Pure.elim_pure_wp_monotonicity_forall ();
+  fun p -> wpV fsG (fun _ -> wpK fsG p)
+
+unfold
+val helper_seq : #g:env ->
+                 ref1:Type0 ->
+                 #wpV:spec_env g (x:unit{ref1}) ->
+                 v:fs_oexp g (x:unit{ref1}) wpV -> (** since this is pure, I don't have to compile it **)
+
+                 #a:Type ->
+                 #wpK:spec_env g a ->
+                 k:fs_oexp g a wpK ->
+                 fs_oexp g a (wp_seq ref1 wpV wpK)
+let helper_seq ref1 v k =
+  FStar.Monotonic.Pure.elim_pure_wp_monotonicity_forall ();
+  fun fsG -> v fsG ; k fsG
+
+[@@no_auto_projectors] // FStarLang/FStar#3986
+noeq
+type compilable : #a:Type -> g:env -> wp:spec_env g a -> fs_oexp g a wp -> Type =
+| CUnit       : #g:env -> compilable g (fun _ p -> p ()) (fun _ -> ())
+| CTrue       : #g:env -> compilable g (fun _ p -> p true) (fun _ -> true)
+| CFalse      : #g:env -> compilable g (fun _ p -> p false) (fun _ -> false)
+
+(** The following three rules for variables should be generalized. What would be an elegant solution? **)
+| CVar0       : #g:env ->
+                #a:Type ->
+                #_:squash (Some? (g 0) /\ a == Some?.v (g 0)) ->
+                compilable #a g _ (helper_var g a 0)
+| CVar1       : #g:env ->
+                #a:Type ->
+                #b:Type ->
+                #_:squash (Some? (g 0) /\ a == Some?.v (g 0)) ->
+ //               compilable #a (extend b g) (fun fsG p -> p (get_v fsG (x+1))) (fun fsG -> get_v fsG (x+1)) ->
+                compilable #a (extend b g) _ (helper_var1 g a b 0)
+| CVar2       : #g:env ->
+                #a:Type ->
+                #b:Type ->
+                #c:Type ->
+                #_:squash (Some? (g 0) /\ a == Some?.v (g 0)) ->
+ //               compilable #a (extend c (extend b g)) (fun fsG p -> p (get_v fsG (x+2))) (fun fsG -> get_v fsG (x+2)) ->
+                compilable #a (extend c (extend b g)) _ (helper_var2 g a b c 0)
+
+| CApp        : #g :env ->
+                #a :Type ->
+                #b :Type ->
+                #wpF : spec_env g (a -> b) ->
+                #f :fs_oexp g (a -> b) wpF ->
+                cf:compilable g wpF f ->
+                #wpX : spec_env g a ->
+                #x :fs_oexp g a wpX ->
+                cx:compilable g wpX x ->
+                compilable g _ (helper_fapp g a b wpF f wpX x)
+
+| CIf         : #g :env ->
+                #a :Type ->
+                #wpC : spec_env g bool ->
+                #c   : fs_oexp g bool wpC ->
+                cc   : compilable g wpC c ->
+                #wpT : spec_env g a ->
+                #t   : fs_oexp g a wpT ->
+                ct   : compilable g wpT t ->
+                #wpE : spec_env g a ->
+                #e   : fs_oexp g a wpE ->
+                ce   : compilable g wpE e ->
+                compilable g _ (helper_if c t e)
+
+| CLambda     : #g :env ->
+                #a :Type ->
+                #b :Type ->
+                #wpBody:spec_env (extend a g) b ->
+                #f :fs_oexp g (a -> b) (wp_lambda wpBody) ->
+                cf:compilable #b (extend a g) wpBody (helper_lambda wpBody f) ->
+                compilable g _ f
+
+| CRefinement : #g:env ->
+                #a:Type ->
+                ref1:(a -> Type0) ->
+                #ref2:(a -> Type0) ->
+                #wpV:spec_env g (x:a{ref1 x}) ->
+                #v:fs_oexp g (x:a{ref1 x}) wpV ->
+                compilable g wpV v ->
+                compilable g _ (helper_ref #g #a #ref1 #ref2 #wpV v)
+
+| CSeq        : #g:env ->
+                ref1:Type0 ->
+                #wpV:spec_env g (x:unit{ref1}) ->
+                #v:fs_oexp g (x:unit{ref1}) wpV ->
+                compilable g wpV v -> (** the name compilable is misleading here.
+                                         I have to compute the WP of `v` to be able to
+                                         compile the entire term **)
+
+                #a:Type ->
+                #wpK:spec_env g a ->
+                #k:fs_oexp g a wpK ->
+                compilable g wpK k ->
+                compilable g _ (helper_seq ref1 v k)
+
+
+let empty_wp #a (wp:spec_env empty a) : pure_wp a =
+  FStar.Monotonic.Pure.elim_pure_wp_monotonicity_forall ();
+  fun p -> forall fsG. wp fsG p
+
+unfold let compilable_closed #a #wp (x:a{forall fsG. wp fsG <= ret x}) =
+  compilable empty wp (fun _ -> x)
+
+let test2_var
+  : compilable (extend unit (extend unit empty)) _ (fun fsG -> get_v (fs_shrink fsG) 0)
+  = CVar1
+
+let test1_exp
+  : compilable_closed #(unit -> unit) (fun x -> x)
+  = CLambda CVar0
+
+let test4_exp'
+  : compilable_closed #(unit -> unit -> unit -> unit) (fun x y z -> y)
+  = CLambda (CLambda (CLambda CVar1))
+
+let test1_hoc
+  : compilable_closed #((bool -> bool) -> bool) (fun f -> f false)
+  = CLambda (CApp CVar0 CFalse)
+
+let test2_if
+  : compilable_closed #(bool -> bool) (fun x -> if x then false else true)
+  = CLambda (CIf CVar0 CFalse CTrue)
+
+let test1_if
+  : compilable_closed #(bool -> bool -> bool) (fun x y -> if x then false else y)
+  = CLambda (CLambda (CIf CVar1 CFalse CVar0))
+
+let test1_comp_ref
+  : compilable_closed #(x:bool{x == true} -> x:bool{x == true}) (fun x -> x)
+  = CLambda CVar0
+
+let test1_erase_ref
+  : compilable_closed #(x:bool{x == true} -> bool) (fun x -> x)
+  = CLambda (CRefinement (fun x -> x == true) CVar0)
+
+open Examples
+
+let test_just_true'
+  : compilable_closed test_just_true
+  = CLambda (CRefinement _ CTrue)
+
+let test_moving_ref'
+  : compilable_closed test_moving_ref
+  = CLambda (CRefinement _ CUnit)
+
+let test_always_false'
+  : compilable_closed test_always_false
+  = CLambda (CRefinement _ (CIf CVar0 (CFalse) CVar0))
+
+let test_always_false''
+  : compilable_closed test_always_false
+  = CLambda (CIf CVar0 (CRefinement (fun _ -> True) CFalse) (CRefinement (fun _ -> True) CVar0))
+
+let test_always_false_complex'
+  : compilable_closed test_always_false_complex
+  = CLambda (CRefinement _ (CIf CVar0 (CIf CVar0 CFalse CTrue) CFalse))
+
+let test_always_false_complex''
+  : compilable_closed test_always_false_complex
+  = CLambda (CIf CVar0 (CIf CVar0 (CRefinement (fun _ -> True) CFalse) (CRefinement (fun _ -> True) CTrue)) (CRefinement (fun _ -> True) CFalse))
+
+let test_if_x'
+  : compilable_closed test_if_x
+  = CLambda (CLambda (CIf CVar0 (CApp CVar1 (CRefinement (fun _ -> True) #(fun x -> x == true) CVar0)) CFalse))
+
+let test_p_implies_q_simpl'
+  : compilable_closed test_p_implies_q_simpl
+  = CLambda (CSeq q_ref (CApp CVar0 CUnit) (CRefinement (fun _ -> True) CUnit))
+  //= CLambda (CApp (CLambda #_ #(_:unit{q_ref}) #(_:unit{q_ref})(CRefinement (fun _ -> True) #(fun _ -> q_ref) CUnit)) (CApp #_ #unit #(_:unit{q_ref}) CVar0 CUnit))
+
+let test_p_implies_q'
+  : compilable_closed test_p_implies_q
+  = CLambda (CLambda (CSeq q_ref (CApp CVar1 CVar0) (CRefinement p_ref CVar0)))
+ // = CLambda (CLambda (CApp (CLambda (CRefinement p_ref #(fun _ -> q_ref) CVar1)) (CApp CVar1 CVar0)))
+
+let test_true_implies_q
+  : compilable_closed test_true_implies_q
+  = CLambda (CLambda (
+     CIf CVar0
+         (CSeq q_ref (CApp CVar1 (CRefinement (fun _ -> True) #(fun x -> x == true) CVar0))
+                     (CRefinement (fun _ -> True) #(fun x -> x == true ==> q_ref) CVar0))
+         (CRefinement (fun _ -> True) #(fun x -> x == true ==> q_ref) CFalse)))
